#матан 
## Задача 1
$\int\limits_{0}^{\infty}x^{\alpha} \cdot e^{-x^\beta} dx = \begin{vmatrix}t = x^{\beta} \\x = t^{\frac{1}{\beta}} \\dx = \frac{1}{\beta} t^{\frac{1}{\beta} - 1}dt \\x^{\alpha} = t^{\frac{\alpha}{\beta}}\end{vmatrix} = \int\limits_{0}^{+ \infty} t^{\frac{\alpha}{\beta}} \cdot e^{-t} \cdot \frac{1}{\beta} \cdot t^{\frac{1}{\beta} - 1} dt = \frac{1}{\beta} \int\limits_{0}^{+ \infty} t^{\frac{\alpha + 1}{\beta} - 1} \cdot e^{-t} dt = \frac{1}{\beta} \cdot Г(\frac{\alpha + 1}{\beta})$
$\alpha > -1$
$\beta > 0$

## Задача 2
$\int\limits_{0}^{+ \infty} \frac{1}{x^{n  +1}} \cdot e^{- \frac{\alpha}{2x^2}}dx = \begin{vmatrix}t = \frac{\alpha}{2x^2} \\x = \sqrt{\frac{\alpha}{2t}} \\dx = - \frac{\sqrt{\alpha}}{2 \sqrt{2t} \cdot t}dt\end{vmatrix} = - \int\limits_{0}^{+ \infty} \frac{1}{(\frac{\alpha}{2t})^{\frac{n + 1}{2}}} \cdot e^{-t} \cdot \frac{\sqrt{\alpha}}{2 \sqrt{2} t^{\frac{3}{2}}} dt =- \frac{\sqrt{\alpha}}{2\sqrt{2}} \int\limits_{0}^{+ \infty} (\frac{2t}{\alpha})^{\frac{n + 1}{2}} \cdot e^{-t} \cdot t^{- \frac{3}{2}}dt =$
$= - \frac{\sqrt{\alpha}}{2^{\frac{3}{2}}} \cdot 2^{\frac{n + 1}{2}} \cdot \frac{1}{\alpha^{\frac{n + 1}{2}}} \cdot \int\limits_{0}^{+ \infty} t^{\frac{n - 2}{2}} \cdot e^{-t} dt = - \frac{\alpha^{\frac{1}{2}}}{\alpha^{\frac{n + 1}{2}}} \cdot 2^{\frac{n}{2} - 1} \int\limits_{0}^{+ \infty} t^{\frac{n}{2} - 1} \cdot e^{-t} dt = - \alpha^{- \frac{n}{2}} \cdot 2^{\frac{n}{2} - 1} \cdot \int\limits_{0}^{+ \infty} t^{\frac{n}{2} - 1} \cdot e^{-t} dt =$
$= \alpha^{- \frac{n}{2}} \cdot 2^{\frac{n}{2} - 1} \cdot Г(\frac{n}{2}) = \frac{2^{\frac{n}{2} - 1}}{\alpha^{\frac{n}{2}}} \cdot Г(\frac{n}{2})$

## Задача 3
$\int\limits_{0}^{1} (\ln(\frac{1}{x}))^{\alpha - 1} \cdot x^{\beta - 1} dx, \ \alpha > 0, \ p > 0$
$\int\limits_{0}^{1} (\ln(\frac{1}{x}))^{\alpha - 1} \cdot x^{\beta - 1} dx = \begin{vmatrix}t = \ln(\frac{1}{x}) \\\frac{1}{x} = e^t \\x = e^{-t} \\dx = e^{-t}\end{vmatrix} = \int\limits_{0}^{\infty} t^{\alpha - 1} e^{-t (\beta - 1)} \cdot e^{-t} dt = \int\limits_{0}^{\infty} t^{\alpha - 1} \cdot e^{-t \beta + t - t} dt = \int\limits_{0}^{\infty} t^{\alpha - 1} e^{-t \beta} dt =$
$= \begin{vmatrix}v = t \beta \\t = \frac{v}{\beta} \\dt = \frac{1}{\beta}\end{vmatrix} = \int\limits_{0}^{\infty} (\frac{v}{\beta})^{\alpha - 1} e^{-v} \frac{1}{\beta} dv = \int\limits_{0}^{\infty} \frac{1}{\beta} \cdot \frac{1}{\beta^{\alpha - 1}} v^{\alpha - 1} e^{-v} dv = \frac{1}{\beta^{\alpha}} Г(\alpha)$

## Задача 4
$\int\limits_{0}^{+ \infty} e^{-e^{x}} \cdot e^{px} dx: \ p > 0$
$\int\limits_{0}^{+ \infty} e^{-e^{x}} \cdot e^{px} dx = \begin{vmatrix}t = e^x \\x = \ln(t) \\dx = \frac{1}{t} dt \\ x: -\infty \to + \infty \\ t: 0 \to + \infty \end{vmatrix} = \int\limits_{0}^{+ \infty} e^{-t} \cdot e^{p \ln(t)} \cdot \frac{dt}{t} = \int\limits_{0}^{+ \infty} t^{p - 1} \cdot e^{-t} dt = Г(p)$

## Задача 5
$\int\limits_{0}^{+ \infty} \frac{dx}{(1 + x^2)^{\alpha}}, \ \alpha > \frac{1}{2}$
$\int\limits_{0}^{+ \infty} \frac{dx}{(1 + x^2)^{\alpha}} = \begin{vmatrix}x^2 = t \\x = \sqrt{t} \\dx = \frac{1}{2} t^{- \frac{1}{2}}dt\end{vmatrix} = \frac{1}{2} \int\limits_{0}^{+ \infty} t^{- \frac{1}{2}} \cdot (1 + t)^{- \alpha} dt = \frac{1}{2} \int\limits_{0}^{+ \infty} t^{\frac{1}{2} - 1}\frac{dt}{(1 + t)^{\frac{1}{2} + \alpha - \frac{1}{2}}} = \frac{1}{2} B(\frac{1}{2}, \alpha - \frac{1}{2})$

## Задача 6
Найти остаток
$I(y) = \int\limits_{0}^{+ \infty} \frac{dx}{1 + x^y}$
$y \in [2; 4]$

$R(A, y) = \int\limits_{A}^{+ \infty} \frac{dx}{1 + x^y} < \int\limits_{A}^{+ \infty} \frac{dx}{1 + x^2} = \frac{\pi}{2} - arctg(A)$

$|\frac{\pi}{2} - arctg(A)| < \varepsilon$
$arctg(A) > \frac{\pi}{2} - \varepsilon$
$A > max \begin{cases} tg(\frac{\pi}{2} - \varepsilon) \\ 0 \end{cases}$

## Задача 7
$\int\limits_{0}^{1} x^{\frac{3}{2}} \cdot (1 - x)^{\frac{1}{2}} dx = \int\limits_{0}^{1} x^{\frac{5}{2} - 1} \cdot (1 - x)^{\frac{3}{2} - 1} dx = \beta(\frac{5}{2}, \frac{3}{2}) = \beta(a, b)$
$\beta(\frac{3}{2} + 1, \frac{3}{2}) = \frac{\frac{3}{2} + 1}{4} \cdot \beta(\frac{3}{2}, \frac{3}{2}) = \frac{\pi}{16}$