#матан 
## Задание 1
$\int\limits_{0}^{+ \infty} \frac{dx}{1 + x^3} = \begin{vmatrix}t = x^3 \\dt = 3x^2 dx \\dx = \frac{dt}{3t^{\frac{2}{3}}} \\t: \ 0 \to + \infty\end{vmatrix} = \int\limits_{0}^{+ \infty} \frac{dt}{3t^{\frac{2}{3}}(1 + t)} = \int\limits_{0}^{+ \infty} \frac{t^{\frac{1}{3} - 1} dt}{(1 + t)^{\frac{1}{3} + \frac{2}{3}}} = \frac{1}{3} \beta(\frac{2}{3}, \frac{1}{3}) = \frac{1}{3} \frac{Г(\frac{2}{3}) Г(\frac{1}{3})}{Г(1)} =$
$= \frac{1}{3} \beta(\frac{1}{3}, \frac{2}{3}) = \frac{1}{3} \beta(\frac{1}{3}, 1 - \frac{2}{3}) = \frac{1}{3} \cdot \frac{\pi}{\sin(\frac{\pi}{3})} = \frac{2 \pi}{3 \sqrt{3}} = \frac{2 \pi \sqrt{3}}{9}$

## Задание 2
$\int\limits_{0}^{\frac{\pi}{2}} \sin^6x \cdot \cos^4 x dx = \begin{vmatrix}t = \sin^2 x \\dt = 2 \sin x \cos x dx \end{vmatrix} = \frac{1}{2} \int\limits_{0}^{1} t^{\frac{7}{2} - 1} (1 - t)^{\frac{5}{2} - 1} dt = \frac{1}{2} \beta(\frac{7}{2}, \frac{5}{2}) = \frac{1}{2} \cdot \frac{Г(\frac{7}{2}) Г(\frac{5}{2})}{Г(6)} =$
1) $Г(\frac{7}{2}) = Г(3 + \frac{1}{2}) = (\frac{1}{2} + 3 - 2)(\frac{1}{2}) Г(\frac{1}{2}) = \sqrt{\pi}$
2) $Г(\frac{5}{2}) = Г(2 + \frac{1}{2}) = \frac{3}{2} \cdot \frac{1}{2} Г(\frac{1}{2})$
3) $Г(5 + 1) = 2^6 \cdot 5!$
$= \frac{3 \pi}{\frac{5}{2}}$

## Задание 3
$\int\limits_{0}^{1} \frac{dx}{\sqrt[n]{1 + x^n}} = \begin{vmatrix}t = x^n \\x = t^{\frac{1}{n}} \\dx = \frac{1}{n} \cdot t^{\frac{1}{n} - 1}dt \end{vmatrix} = \frac{1}{n} \int\limits_{0}^{1} \frac{t^{\frac{1}{n} - 1} dt}{(1 + t)^{\frac{1}{n}}} = \frac{1}{n} \int\limits_{0}^{1} (1 + t)^{(1 - \frac{1}{n}) - 1} \cdot t^{\frac{1}{n} - 1} dt = \frac{1}{n} \beta(1 - \frac{1}{n}, \frac{1}{n}) = \frac{1}{n} \cdot \frac{\pi}{\sin(\frac{\pi}{n})}$

## Задание 4
$\int\limits_{0}^{\frac{\pi}{2}} tg^n (x) dx = \begin{vmatrix}tg(x) = \sqrt{t} \\x = arctg(\sqrt{t}) \\dx = \frac{1}{t + 1} \cdot \frac{1}{2 \sqrt{t}} dt \end{vmatrix} = \int\limits_{0}^{+ \infty} \frac{t^{\frac{n}{2}} dt}{(t + 1) 2t^{\frac{1}{2}}} = \int\limits_{0}^{+ \infty} \frac{t^{\frac{n - 1}{2}} dt}{t + 1} = \frac{1}{2} \int\limits-{0}^{+ \infty} \frac{t^{(\frac{n - 1}{2} + 1) - 1}}{t + 1} dt =$
$= \frac{1}{2} \beta(\frac{n - 1}{2} + 1, 1 - \frac{n - 1}{2} - 1) = \frac{1}{2} \beta(\frac{n + 1}{2}, \frac{1 - n}{2}) = \frac{1}{2} \cdot \frac{\pi}{\sin(\frac{n - 1}{2} + 1) \pi} = \frac{1}{2} \cdot \frac{\pi}{\sin(\frac{n + 1}{2}) \pi} = \frac{\pi}{2 \cos(\frac{\pi n}{2})}$
Сходится, если $|n| < 1$

## Задание 5
$\int\limits_{0}^{1} (\ln(\frac{1}{x}))^p dx = \begin{vmatrix}t = \ln(\frac{1}{x}) \\x = \frac{1}{e^t} \\ dx = - \frac{1}{e^t} dt \end{vmatrix} = - \int\limits_{+ \infty}^{0} t^p \frac{1}{e^t} dt = \int\limits_{0}^{+ \infty} t^p \cdot e^{-t} \cdot dt = Г(p + 1)$

## Задание 6
$\int\limits_{0}^{\frac{\pi}{2}} \sin^{\frac{5}{2}} x \cos^{\frac{3}{2}} x dx = \frac{1}{2} \int\limits_{0}^{\frac{\pi}{2}} \sin(2x) \cdot \sin^{\frac{3}{2}} x \cdot \cos^{\frac{1}{2}} x \ dx = \begin{vmatrix}t = \sin^2 x \\dt = \sin 2x dx \end{vmatrix} = \frac{1}{2} \int\limits_{0}^{1} t^{\frac{3}{4}} \cdot (1 - t)^{\frac{1}{4}} dt = \frac{1}{2} \beta(\frac{7}{4}, \frac{5}{4}) =$
$= \frac{1}{2} \cdot \frac{Г(\frac{7}{4}) Г(\frac{5}{4})}{Г(3)} = \frac{1}{4} \cdot \frac{3}{4} \cdot \frac{1}{4} \cdot \frac{Г(\frac{3}{4}) Г(\frac{1}{4})}{Г(1)} = \frac{3}{2^6} \cdot \beta(\frac{1}{4}, 1 - \frac{1}{4}) = \frac{3}{2^6} \cdot \frac{\pi}{\sin(\frac{\pi}{4})} = \frac{3 \sqrt{2} \pi}{64}$