#матан 
## Задание 1
$\int\limits_{L} xy^2 dx + yx^2 dy $
$L: \ \frac{x^2}{a^2} + \frac{y^2}{b^2} = 1$ - часть в 1-ой четверти

$x = a \cos t \implies dx = - a \sin dt$
$y = b \sin t \implies dy = b \cos dt$
$t \in [0; \frac{\pi}{2}]$

Тогда:
$\int\limits_{L} xy^2 dx + yx^2 dy = \int\limits_{0}^{\frac{\pi}{2}} [(a \cos t b^2 \sin^2 t) a \sin dt + (b \sin t a^2 \cos^2 t) b \cos dt] =$
$= a^2 b^2 \int \limits_{0}^{\frac{\pi}{2}} (\sin t \cos^3 t - \cos t \sin^3 t)dt = a^2 b^2 (\frac{\sin^4 t}{4} + \frac{\cos^4 t}{4})|_{0}^{\frac{\pi}{2}} = a^2 b^2 (\frac{1}{4} - 0 + 0 - \frac{1}{4}) = 0$

## Задание 2
$\int\limits_{L} xy dx + (x + y)dy$

$L: \ O(0, 0), A(1, 1)$
а) $y = x$
б) $y = x^2$
в) $x = y^2$
г) $y = x^3$
д) OBA, B(1, 0)

а) $\int\limits_{0}^{1} (x^2 + x) dx = \frac{x^3}{3} + x^2|_{0}^{1} = \frac{4}{3}$
б) $\int\limits_{0}^{1} (x^3 + 2x^2 + 2x^3) dx = (\frac{3x^4}{4} + \frac{2x^3}{3})|_{0}^{1} = \frac{3}{4} + \frac{2}{3} = \frac{17}{12}$
в) $\int\limits_{0}^{1} (y^3 \cdot 2y + y^2 + y)dy = (\frac{2 y^5}{5} + \frac{y^3}{3} + \frac{y^2}{2})|_{0}^{1} = \frac{2}{5} + \frac{1}{3} + \frac{1}{2} = \frac{37}{30}$
	$x = y^2$
	$dx = 2y dy$
г) $dy = 3x^2 dx$
	$\int\limits_{0}^{1} (x^4 + (x + x^3) \cdot 3x^2) dx = \int\limits_{0}^{1} 3x^5 + x^4 + 3x^3 dx = (\frac{x^6}{2} + \frac{x^5}{5} + \frac{3x^4}{4})|_{0}^{1} = \frac{29}{20}$
д) $0 + \int\limits_{0}^{1} 1 + y dy = \int\limits_{0}^{1} y + 1 dy = (\frac{y^2}{2} + y)|_{0}^{1} = \frac{3}{2}$

## Задание 3
$\int\limits_{L} (x + y)ds$, где $L = AB$ циклоиды^
- $x = a(t - \sin t)$
- $y = a(1 - \cos t)$
- $A = (0; 0)$
- $B = (4 \pi a; 0)$
![[Pasted image 20250523115343.png|400]]

$ds = \sqrt{(x')^2 + (y')^2}dt$
$x' = a(1 - \cos t)$
$y' = a \sin t$
$ds = a \sqrt{(1 - \cos t)^2 + \sin^2 t} dt = a \sqrt{2 - 2 \cos t}dt = a \sqrt{2} \sqrt{1 - \cos t} =$
$= a \sqrt{2} \sqrt{2 \sin^2 \frac{t}{2}} dt = 2a |\sin \frac{t}{2}| dt$

$2a^2 (t - \sin t + 1 - \cos t) \cdot |\sin \frac{t}{2}| dt = 2a^2 (t - 2 \sin \frac{t}{2} \cos \frac{t}{2} + 2 \sin^2 \frac{t}{2}) \cdot |\sin \frac{t}{2}|dt$

$2a^2(\int\limits_{0}^{2 \pi} (t - 2 \sin \frac{t}{2} \cos \frac{t}{2} + 2 \sin^2 \frac{t}{2}) \sin \frac{t}{2} dt - \int\limits_{2 \pi}^{4 \pi} (t - 2 \sin \frac{t}{2} \cos \frac{t}{2} + 2 \sin^2 \frac{t}{2}) \sin \frac{t}{2} dt) =$
$= 2a^2 ()$ ну и хуяку забили

## Задание 4