#матан 
## Задание 1
$\int\limits_{0}^{+ \infty} \frac{\sqrt[4]{x}dx}{(1 + x)^2} = \int\limits_{0}^{+ \infty} \frac{x^{5/4} - 1}{(1 + x)^{5/4 + 3/4}} = B(5/4; 3/4) = \frac{Г(5/4) Г(3/4)}{Г(2)} = Г(1/4 + 1) Г(3/4) = \frac{1}{4} Г(3/4) Г(1/4) = \frac{1}{4} \frac{\pi}{\sin \frac{3 \pi}{4}} = \frac{\pi}{2 \sqrt{2}}$

## Задание 2
$\int\limits_{0}^{\infty} = \begin{vmatrix}x = \sqrt[4]{t} \\dx = \frac{1}{4 t^{3/4}}dt\end{vmatrix} \int\limits_{0}^{\infty} \frac{t^{1/2}}{1 + t} \cdot \frac{1}{4t^{3/4}}dt = \frac{1}{4} \int\limits_{0}^{\infty} \frac{}{}$
ДОПИСАТЬ
## Задание 3
$\int\limits_{0}^{+ \infty} x^{2n} e^{-x^2} dx = \begin{vmatrix}t = x^2 \\x = \sqrt{t} \\dx = \frac{1}{2} \cdot \frac{1}{\sqrt{t}} dt\end{vmatrix} = \frac{1}{2} \int\limits_{0}^{+ \infty} t^n \cdot e^{-t} \cdot \frac{dt}{\sqrt{t}} = \frac{1}{2} \int\limits_{0}^{+ \infty} t^{(n + \frac{1}{2}) - 1} e^{-t} dt = \frac{1}{2} Г(n + \frac{1}{2}) =$
$= \frac{1}{2} (\frac{1}{2} + n - 1) \cdot \dots \frac{1}{2} Г(\frac{1}{2}) = \frac{1}{2} (- \frac{1}{2} + n) \cdot \dots \frac{1}{2} \sqrt{n} = \frac{1}{2} \sqrt{\pi} \cdot (n - \frac{1}{2}) \cdot (n - \frac{3}{2}) \cdot \dots \frac{1}{2} = \frac{\frac{1}{2} \sqrt{\pi} \cdot (2n - 1)!!}{2n + 1}$

## Задание 4
$\int\limits_{0}^{\frac{\pi}{2}} \sin^{p - 1}(x) \cdot \cos^{q - 1}(x) dx, p, q > 0$
$\begin{vmatrix}t = \sin^2 x \\dt = 2 \sin x \cdot \cos x dx = \sin 2x dx \\\sin x = t^{\frac{1}{2}} \\\cos x = (1 - t)^{\frac{1}{2}}\end{vmatrix} = \int\limits_{0}^{1} \frac{(t^{\frac{1}{2}})^{p - 1} \cdot ((1 - t)^{\frac{1}{2}})^{q - 1}}{2 t^{\frac{1}{2}} (1 - t)^{\frac{1}{2}}} dt = \frac{1}{2} \int\limits_{0}^{1} t^{\frac{p}{2} - 1} \cdot (1 - t)^{\frac{q}{2} - 1} dt = \frac{B}{2}(\frac{p}{2}; \frac{q}{2}) = \frac{1}{2} \frac{Г(\frac{p}{2}) Г(\frac{q}{2})}{Г(\frac{p + q}{2})}$

При $q = 1: \frac{\sqrt{\pi}}{2} \cdot \frac{Г(\frac{p}{2})}{Г(\frac{p + 1}{2})}$

## Задание 5
$\int\limits_{0}^{\frac{\pi}{2}} \sin^{\alpha}x \cdot \cos^{\beta}x dx, \alpha > -1, \beta > -1$
$\begin{vmatrix}t = \sin^2 x \\dt = 2 \sin x \cos x dx = 2 t^{\frac{1}{2}} (1 - t)^{\frac{1}{2}} dt \\\sin x = t^{\frac{1}{2}} \\\cos x = (1 - t)^{\frac{1}{2}}\end{vmatrix} = \int\limits_{0}^{1} \frac{t^{\alpha/2} \cdot (1 - t)^{\beta/2}}{2t^{\frac{1}{2}}(1 - t)^{\frac{1}{2}}} dt = \frac{1}{2} \int\limits_{0}^{1} t^{\frac{\alpha - 1}{2}} \cdot (1 - t)^{\frac{\beta - 1}{2}} dt = \frac{1}{2} B(\frac{\alpha + 1}{2}; \frac{\beta + 1}{2}) = \frac{1}{2} \frac{Г(\frac{\alpha + 1}{2}) Г(\frac{\beta + 1}{2})}{Г(\frac{\alpha + \beta}{2} + 1)}$

## Задание 6
$\int\limits_{0}^{1} (1 - x^p)^{- \frac{1}{p}} dx = \begin{vmatrix}1 - x^p = t \\1 - t = x^p \\x = (1 - t)^{\frac{1}{p}} \\ dx = - \frac{1}{p} (1 - t)^{\frac{1}{p} - 1} \end{vmatrix} = - \int\limits_{1}^{0} \frac{(1 - t)^{\frac{1}{p} - 1}}{p} \cdot t^{- \frac{1}{p}} dt = \frac{1}{p} \int\limits_{0}^{1} (1 - t)^{\frac{1}{p} - 1} \cdot t^{(- \frac{1}{p} + 1) - 1} dt = \frac{1}{p} B(\frac{1}{p}; - \frac{1}{p} + 1)$
$\frac{1}{p} \in (0, 1)$

## Задание 7
$\int\limits_{0}^{2} \frac{dx}{\sqrt[3]{x^2 \cdot (2 - x)}} = \begin{vmatrix}x = 2t \\dx = 2 dt\end{vmatrix} = 2 \int\limits_{0}^{1} \frac{dt}{\sqrt[3]{4t^2 \cdot 2(1 - t)}} = \int\limits_{0}^{1} \frac{dt}{t^{2/3} (1- t)^{1/3}} = \int\limits_{0}^{1} t^{- 2/3} \cdot (1 - t)^{- 1/3} dt = B(\frac{1}{3}; \frac{2}{3}) = \frac{\pi}{\sin \frac{\pi}{3}} = \frac{2 \pi \sqrt{3}}{3}$

# Интегралы с параметром
## Задание 1
Вычислить: $\int\limits_{0}^{2} \frac{dx}{\sqrt[5]{x^3 \cdot (2 - x)^{2}}} = \begin{vmatrix}x = 2t \implies x: 0 \to 2 \\dx = 2dt \implies t: 0 \to 1\end{vmatrix} = \int\limits_{0}^{1} \frac{2dt}{\sqrt[5]{8t^3 (2 - 2t)^2}} = \int\limits_{0}^{1} \frac{dt}{t^{3/5} (1- t)^{2/5}} = \int\limits_{0}^{1}t^{-3/5} (1- t)^{-2/5} dt = B(\frac{2}{5}; \frac{3}{5}) = \frac{\pi}{\sin \frac{2\pi}{5}}$

## Задание 2
Исследовать на сходимость в зависимости от p, $q > 0$
$\int\limits_{0}^{+ \infty} \frac{x^{p - 1}}{1 + x^q} = \begin{vmatrix}x^q = t \\x = t^{\frac{1}{q}} \\dx = \frac{1}{q} t^{\frac{1 - q}{q}}dt\end{vmatrix} = \frac{1}{q} \int\limits_{0}^{+ \infty} \frac{t^{\frac{p - 1}{q}} \cdot t^{\frac{1 - q}{q}}}{1 + t} = \frac{1}{q} \int\limits_{0}^{+ \infty} \frac{t^{\frac{p - q}{q}}}{1 + t} dt = \frac{1}{q} \int\limits_{0}^{+ \infty} \frac{t^{\frac{p}{q} - 1}}{1 + t} dt = \frac{1}{q} \int\limits-{0}^{+ \infty} t^{\frac{p}{q} - 1} \cdot (1 + t)^{-1} dt = \frac{1}{q} B(\frac{p}{q}; 1 - \frac{p}{q})$
Сходится при $p \in (0; q), \ \frac{p}{q} \in (0; 1)$

## Задание 3
$\int\limits_{-1}^{2} \frac{dx}{\sqrt[4]{(2 - x)(1 + x)^3}} = \begin{vmatrix}1 + x = 3t \\ x = 3t - 1 \\dx = 3dt\end{vmatrix} = \int\limits_{0}^{1} \frac{3dt}{\sqrt[4]{(3 - 3t)(3t)^3}} = 3 \int\limits_{0}^{1} \frac{dt}{3 \sqrt[4]{(1 - t)t^3}} = \int\limits_{0}^{1} (1 - t)^{-1/4} t^{-3/4} dt = B(\frac{3}{4}; \frac{1}{4}) = \frac{Г(\frac{3}{4}) Г(\frac{1}{4})}{Г(1)} = \frac{\pi}{\sin(- \frac{\pi}{4})} = \frac{\pi}{\frac{\sqrt{2}}{2}} = \sqrt{2} \pi$

## Задание 4
$\int\limits_{0}^{2} \frac{dx}{\sqrt[4]{(2 + x)^3 (2 - x)}} = \begin{vmatrix}t = \frac{x + 2}{4} \\4t - 2 = x \\dx = 4dt\end{vmatrix} = \int\limits_{0}^{1} \frac{4 dt}{\sqrt[4]{(4t)^3 (4 - 4t)}} = B(\frac{1}{4}; \frac{3}{4}) = \frac{\pi}{\sin(\frac{\pi}{4})} = \pi \sqrt{2}$

## Задание 5
$\int\limits_{1}^{2} \sqrt[3]{(2 - x)^2 (x - 1)}dx = \begin{vmatrix}t = x - 1 \implies x \to 1 \\x = t + 1 \implies 1 \to 0\end{vmatrix} \int\limits_{0}^{1} \sqrt[3]{(1 - t)^2 \cdot t}dt = \int\limits_{0}^{1} t^{1/3} (1 - t)^{2/3} dt = \int\limits_{0}^{1} t^{\frac{4}{3} - 1} (1 - t)^{\frac{5}{3} - 1}dt = B(\frac{4}{3}; \frac{5}{3}) = \frac{Г(\frac{4}{3}) Г(\frac{5}{3})}{Г(3)} = \frac{1}{9} \cdot \frac{\pi}{\sin \frac{\pi}{3}} = \frac{2}{9\sqrt{3}} \pi$

## Задание 6
$\int\limits_{1}^{2} \sqrt{\frac{x - 1}{2 - x}} \cdot \frac{dx}{(x + 3)^2} = \begin{vmatrix}t = \frac{x - 1}{2 - x} = -1 + \frac{1}{2 - x} \\t + 1 = \frac{1}{2 - x}; \ x = 2 - \frac{1}{t + 1} \\dx = \frac{dt}{(t + 1)^2}\end{vmatrix} = \int\limits_{0}^{+ \infty} \frac{dt\sqrt{t} }{(t + 1)^2 (5 - \frac{1}{t + 1})^2} = \int\limits_{0}^{+ \infty} = \int\limits_{0}^{+ \infty} \frac{\sqrt{t} dt}{(5(t + 1) - 1)^2} = \int\limits_{0}^{+ \infty} \frac{\sqrt{t} dt}{(5t + 4)^2} =$
$= \frac{1}{16} \int\limits_{0}^{+ \infty} \frac{\sqrt{t} dt}{(\frac{5}{4} t + 1)^2} = \frac{1}{16} \int\limits_{0}^{+ \infty} \frac{\sqrt{\frac{4}{5}} \sqrt{\frac{5}{4}t} dt}{(\frac{5}{4} t + 1)^2} = \begin{vmatrix}\sqrt{\frac{5}{4} t} = u \\t = \frac{4u^2}{5} \\dt = \frac{4}{5} 2 udu\end{vmatrix} = \frac{1}{10 \sqrt{5}} \int\limits_{0}^{+ \infty} \frac{\sqrt{u} du}{(u + 1)^2} = \frac{1}{10 \sqrt{5}} B(\frac{3}{2}; \frac{1}{2}) = \frac{1}{10 \sqrt{5}} \frac{Г(\frac{3}{2}) Г(\frac{1}{2})}{Г(2)} =$
$= \frac{1}{10 \sqrt{5}} \frac{\frac{1}{2} (Г(\frac{1}{2}))^2}{1} = \frac{1}{10 \sqrt{5}} \cdot \frac{1}{2} \cdot \pi = \frac{\pi}{20 \sqrt{5}}$

## Задание 7
ДОПИСАТЬ

## Задание 8
$\int\limits_{0}^{\frac{\pi}{2}} \cos^{\alpha} x \cdot \cos^{\beta} x dx = \begin{vmatrix}t = \sin^2 x \\dt = 2 \cos x \sin x dx \\dx = \frac{dt}{2 \sqrt{t} \sqrt{1 - t}}\end{vmatrix} = \int\limits_{0}^{1} (1 - t)^{\frac{\alpha}{2}} (1 - t)^{\frac{\beta}{2}} \cdot \frac{dt}{2 \sqrt{t} \sqrt{1 - t}} = \frac{1}{2} \int\limits_{1}^{0} (1 - t)^{\frac{\alpha + \beta - 1}{2}} t^{- \frac{1}{2} dt} = \frac{1}{2} \int\limits_{0}^{1} (1 - t)^{\frac{\alpha + \beta + 1}{2} - 1} t^{\frac{1}{2} - 1} = \frac{B(\frac{\alpha + \beta + 1}{2}; \frac{1}{2})}{2} =$
$= \frac{1}{2} \cdot \frac{Г(\frac{\alpha + \beta + 1}{2}) Г(\frac{1}{2})}{Г(\frac{\alpha + \beta + 2}{2})} = \frac{\sqrt{\pi}}{2} \cdot \frac{Г(\frac{\alpha + \beta + 1}{2})}{Г(\frac{\alpha + \beta}{2} + 1)} = |\frac{\alpha + \beta}{2} = p| = \frac{\sqrt{\pi}}{2} \cdot \frac{Г(p + \frac{1}{2})}{Г(p + 1)} = \frac{\sqrt{\pi}}{2} \cdot \frac{Г(p + \frac{1}{2})}{pГ(p)}$