#диффуры 
$$\begin{cases} y_1' = a y_1 + b y_2 \\ y_2' = c y_1 + b y_2 \end{cases}$$
$$\frac{d}{dt} \begin{pmatrix}y_1 \\y_2\end{pmatrix} = \begin{pmatrix}a & b \\c & d\end{pmatrix} \cdot \begin{pmatrix}y_1 \\y_2\end{pmatrix}$$
Либо, если $y = \begin{pmatrix}y_1 \\y_2\end{pmatrix}, \ A = \begin{pmatrix}a & b \\c & d\end{pmatrix}$, тогда:
$$\frac{d}{dt}y = Ay$$
Пусть $u = u(t), \ b_1, b_2$ - не зависят от t, тогда:
$$u'' + b_1 u' + b_2 u' = 0$$
$u = e^{\lambda \cdot t} \cdot u_0$
$\lambda^2 u  + b_1 \lambda u + b_2 u = 0$
$(\lambda^2 + b_1 \lambda + b_2) \cdot u(t) = 0$
$$y = e^{\lambda t} \cdot v$$
$$\lambda v e^{\lambda t} = A e^{\lambda t} v$$
$$Av = vt$$
$(A)(v) = \lambda (v)$

$\begin{cases} y_1'' = ay_1 + by_2 \ (1) \\ y_2 = \frac{1}{b} (y_1' - ay_1) \ (2) \end{cases}$

Из начала взяли: $y_2' = cy_1 + by_2$
Из (2) получаем: $y_1'' = ay_2' + b(cy_2 + b \cdot \frac{1}{b} (y_1' - ay_1))$
Тогда:
$$y_1'' = (a + b)y_1' + bcy_1 - bay_1$$

$$\frac{d}{dt}X(t) = AX(t)$$
$$X(t) = V \cdot e^{\lambda t}$$
$$A \cdot V = \lambda V$$
$$(A - \lambda I)V = 0$$